

 Expand $(a-2b+c)+(-2a+b-3c)$:


\ifsat
	\begin{enumerate}[label=\Alph*)]
		\item   $-a-b-2c$%
		\item  $-a+b-c$
		\item  $a-b-c$
		\item   $-a-b-c$
	\end{enumerate}
\else
\fi

\ifacteven
	\begin{enumerate}[label=\textbf{\Alph*.},itemsep=\fill,align=left]
		\setcounter{enumii}{5}
		\item   $-a-b-2c$%
		\item  $a+2b-c$
		\item  $-a+b-c$
		\addtocounter{enumii}{1}
		\item  $a-b-c$
		\item   $-a-b-c$
	\end{enumerate}
\else
\fi

\ifactodd
	\begin{enumerate}[label=\textbf{\Alph*.},itemsep=\fill,align=left]
		\item   $-a-b-2c$%
		\item  $a+2b-c$
		\item  $-a+b-c$
		\item  $a-b-c$
		\item   $-a-b-c$
	\end{enumerate}
\else
\fi

\ifgridin
   $-a-b-2c$%
		
\else
\fi

