


  Which of the following expressions equals $(x+5)(x-3)$?


\ifsat
	\begin{enumerate}[label=\Alph*)]
		\item   $x^2-2x-15$%
		\item  $x^2+2x-15$
		\item  $x^2-2x+15$
		\item  $x^2-8x+15$
	\end{enumerate}
\else
\fi

\ifacteven
	\begin{enumerate}[label=\textbf{\Alph*.},itemsep=\fill,align=left]
		\setcounter{enumii}{5}
		\item   $x^2-2x-15$%
		\item  $x^2+2x-15$
		\item  $x^2-2x+15$
		\addtocounter{enumii}{1}
		\item  $x^2+2x+15$
		\item  $x^2-8x+15$
	\end{enumerate}
\else
\fi

\ifactodd
	\begin{enumerate}[label=\textbf{\Alph*.},itemsep=\fill,align=left]
		\item   $x^2-2x-15$%
		\item  $x^2+2x-15$
		\item  $x^2-2x+15$
		\item  $x^2+2x+15$
		\item  $x^2-8x+15$
	\end{enumerate}
\else
\fi

\ifgridin
   $x^2-2x-15$%
		
\else
\fi

