 
$(j+k)^2-(k-j)^2$


\ifsat
	\begin{enumerate}[label=\Alph*)]
		\item $0$
		\item $2j^2$
		\item $4jk$ % 
		\item $2j^2+2k^2$
	\end{enumerate}
\else
\fi

\ifacteven
	\begin{enumerate}[label=\textbf{\Alph*.},itemsep=\fill,align=left]
		\setcounter{enumii}{5}
		\item $0$
		\item $2j^2$
		\item $4jk$ % 
		\addtocounter{enumii}{1}
		\item $2j^2+2k^2$
		\item None of these. 
	\end{enumerate}
\else
\fi

\ifactodd
	\begin{enumerate}[label=\textbf{\Alph*.},itemsep=\fill,align=left]
		\item $0$
		\item $2j^2$
		\item $4jk$ % 
		\item $2j^2+2k^2$
		\item None of these. 
	\end{enumerate}
\else
\fi

\ifgridin
 $4jk$ % 
		
\else
\fi

