



 Which of the following is the same as $(2x+y-z)-(x-y+z)$?


\ifsat
	\begin{enumerate}[label=\Alph*)]
		\item  $x+2y+2z$
		\item  $x+2y-2z$%
		\item  $x-2y+2z$
		\item  $x-2y-2z$
	\end{enumerate}
\else
\fi

\ifacteven
	\begin{enumerate}[label=\textbf{\Alph*.},itemsep=\fill,align=left]
		\setcounter{enumii}{5}
		\item  $x+2y+2z$
		\item  $x+2y-2z$%
		\item  $x-2y+2z$
		\addtocounter{enumii}{1}
		\item  $x-2y-2z$
		\item  $x+y-2z$
	\end{enumerate}
\else
\fi

\ifactodd
	\begin{enumerate}[label=\textbf{\Alph*.},itemsep=\fill,align=left]
		\item  $x+2y+2z$
		\item  $x+2y-2z$%
		\item  $x-2y+2z$
		\item  $x-2y-2z$
		\item  $x+y-2z$
	\end{enumerate}
\else
\fi

\ifgridin
  $x+2y-2z$%
		
\else
\fi

