 
$$625g^4-h^4 $$
Which of the following is equivalent to the expression shown above?  (Note: $i=\sqrt{-1}$)


\ifsat
	\begin{enumerate}[label=\Alph*)]
		\item $(5g-h)^4 $ 
		\item $(5g^2+ih^2)^2 $ 
		\item $(5g-h)^2(5g+h)^2 $ 
		\item $(5g+ih)(5g-ih)(5g+h)(5g-h) $ % 
	\end{enumerate}
\else
\fi

\ifacteven
	\begin{enumerate}[label=\textbf{\Alph*.},itemsep=\fill,align=left]
		\setcounter{enumii}{5}
		\item $(5g-h)^4 $ 
		\item $(5g^2+ih^2)^2 $ 
		\item $(5g-h)^2(5g+h)^2 $ 
		\addtocounter{enumii}{1}
		\item $(5g+ih)(5g-ih)(5g+h)(5g-h) $ % 
		\item None of these. 
	\end{enumerate}
\else
\fi

\ifactodd
	\begin{enumerate}[label=\textbf{\Alph*.},itemsep=\fill,align=left]
		\item $(5g-h)^4 $ 
		\item $(5g^2+ih^2)^2 $ 
		\item $(5g-h)^2(5g+h)^2 $ 
		\item $(5g+ih)(5g-ih)(5g+h)(5g-h) $ % 
		\item None of these. 
	\end{enumerate}
\else
\fi

\ifgridin
 $(5g+ih)(5g-ih)(5g+h)(5g-h) $ % 

\else
\fi

