 
Simplify:
$$ (x+2)(x^2-2x+4) - (x-1)(x^2-2x+1)$$


\ifsat
	\begin{enumerate}[label=\Alph*)]
		\item $-3x^2+3x-9 $ 
		\item $3x^2-3x-7 $ % 
		\item $x^2-2x+7 $ 
		\item $9$
	\end{enumerate}
\else
\fi

\ifacteven
	\begin{enumerate}[label=\textbf{\Alph*.},itemsep=\fill,align=left]
		\setcounter{enumii}{5}
		\item $-3x^2+3x-9 $ 
		\item $3x^2-3x-7 $ % 
		\item $x^2-2x+7 $ 
		\addtocounter{enumii}{1}
		\item $x^2+x+7 $
		\item $9$
	\end{enumerate}
\else
\fi

\ifactodd
	\begin{enumerate}[label=\textbf{\Alph*.},itemsep=\fill,align=left]
		\item $-3x^2+3x-9 $ 
		\item $3x^2-3x-7 $ % 
		\item $x^2-2x+7 $ 
		\item $x^2+x+7 $
		\item $9$
	\end{enumerate}
\else
\fi

\ifgridin
 $3x^2-3x-7 $ % 
		
\else
\fi

