

 Simplify: $(x+y)^2-(x-y)^2$


\ifsat
	\begin{enumerate}[label=\Alph*)]
		\item   $x^2+y^2$
		\item  $xy$
		\item  $2xy$
		\item  $4xy$%
	\end{enumerate}
\else
\fi

\ifacteven
	\begin{enumerate}[label=\textbf{\Alph*.},itemsep=\fill,align=left]
		\setcounter{enumii}{5}
		\item   $x^2+y^2$
		\item  $xy$
		\item  $2xy$
		\addtocounter{enumii}{1}
		\item   $3xy$
		\item  $4xy$%
	\end{enumerate}
\else
\fi

\ifactodd
	\begin{enumerate}[label=\textbf{\Alph*.},itemsep=\fill,align=left]
		\item   $x^2+y^2$
		\item  $xy$
		\item  $2xy$
		\item   $3xy$
		\item  $4xy$%
	\end{enumerate}
\else
\fi

\ifgridin
  $4xy$%

\else
\fi

