 
For all $x\leq -2$, let the function $g$ be defined as
$g(x)=\sqrt{-6-3x}$.  Which of the following correctly represents the inverse function $g^{-1}(x)$?


\ifsat
	\begin{enumerate}[label=\Alph*)]
		\item $g^{-1}(x)=${\Large$\frac{x-6}{3}$}, $x\geq0 $
		\item $g^{-1}(x)=-\sqrt{-6-3x}, x\leq-2 $
		\item $g^{-1}(x)=${\Large $\frac{x^2+6}{-3}$}, $x\geq0 $ % 
		\item $g^{-1}(x)=${\Large $\frac{x^2-6}{3}$}, $x\geq0$
	\end{enumerate}
\else
\fi

\ifacteven
	\begin{enumerate}[label=\textbf{\Alph*.},itemsep=\fill,align=left]
		\setcounter{enumii}{5}
		\item $g^{-1}(x)=${\Large$\frac{x-6}{3}$}, $x\geq0 $
		\item $g^{-1}(x)=-\sqrt{-6-3x}, x\leq-2 $
		\item $g^{-1}(x)=${\Large$\frac{\sqrt{-6-3x}}{-6-3x}$}, $x\leq-2 $
		\addtocounter{enumii}{1}
		\item $g^{-1}(x)=${\Large $\frac{x^2+6}{-3}$}, $x\geq0 $ % 
		\item $g^{-1}(x)=${\Large $\frac{x^2-6}{3}$}, $x\geq0$
	\end{enumerate}
\else
\fi

\ifactodd
	\begin{enumerate}[label=\textbf{\Alph*.},itemsep=\fill,align=left]
		\item $g^{-1}(x)=${\Large$\frac{x-6}{3}$}, $x\geq0 $
		\item $g^{-1}(x)=-\sqrt{-6-3x}, x\leq-2 $
		\item $g^{-1}(x)=${\Large$\frac{\sqrt{-6-3x}}{-6-3x}$}, $x\leq-2 $
		\item $g^{-1}(x)=${\Large $\frac{x^2+6}{-3}$}, $x\geq0 $ % 
		\item $g^{-1}(x)=${\Large $\frac{x^2-6}{3}$}, $x\geq0$
	\end{enumerate}
\else
\fi

\ifgridin
 $g^{-1}(x)=${\Large $\frac{x^2+6}{-3}$}, $x\geq0 $ % 
		
\else
\fi

