 
Simplify:
$$ \frac{x+7}{x+1}-\frac{x-1}{x+7} $$


\ifsat
	\begin{enumerate}[label=\Alph*)]
		\item {\Large $\frac{48}{x^2+7}  $ }
		\item $-1$
		\item {\Large$\frac{2(7x+24)}{(x+1)(x+7)}  $}
		\item {\Large$\frac{2(7x+25)}{(x+1)(x+7)} $} % 
	\end{enumerate}
\else
\fi

\ifacteven
	\begin{enumerate}[label=\textbf{\Alph*.},itemsep=\fill,align=left]
		\setcounter{enumii}{5}
		\item {\Large $\frac{48}{x^2+7}  $ }
		\item $-1$
		\item {\Large$\frac{2(7x+24)}{(x+1)(x+7)}  $}
		\addtocounter{enumii}{1}
		\item {\Large$\frac{2(7x+25)}{(x+1)(x+7)} $} % 
		\item {\Large$\frac{2-x^2}{x+1}$}
	\end{enumerate}
\else
\fi

\ifactodd
	\begin{enumerate}[label=\textbf{\Alph*.},itemsep=\fill,align=left]
		\item {\Large $\frac{48}{x^2+7}  $ }
		\item $-1$
		\item {\Large$\frac{2(7x+24)}{(x+1)(x+7)}  $}
		\item {\Large$\frac{2(7x+25)}{(x+1)(x+7)} $} % 
		\item {\Large$\frac{2-x^2}{x+1}$}
	\end{enumerate}
\else
\fi

\ifgridin
 {\Large$\frac{2(7x+25)}{(x+1)(x+7)} $} % 

\else
\fi

