



  Simplify: \[(-2x^{2}y^{3})^{3}\]



\ifsat
	\begin{enumerate}[label=\Alph*)]
		\item   $-2x^{6}y^{9}$
		\item  $-8x^{5}y^{6}$
		\item  $-8x^{6}y^{9}$%
		\item   $8x^{6}y^{9}$
	\end{enumerate}
\else
\fi

\ifacteven
	\begin{enumerate}[label=\textbf{\Alph*.},itemsep=\fill,align=left]
		\setcounter{enumii}{5}
		\item   $-2x^{6}y^{9}$
		\item  $-8x^{5}y^{6}$
		\item  $-8x^{6}y^{6}$
		\addtocounter{enumii}{1}
		\item  $-8x^{6}y^{9}$%
		\item   $8x^{6}y^{9}$
	\end{enumerate}
\else
\fi

\ifactodd
	\begin{enumerate}[label=\textbf{\Alph*.},itemsep=\fill,align=left]
		\item   $-2x^{6}y^{9}$
		\item  $-8x^{5}y^{6}$
		\item  $-8x^{6}y^{6}$
		\item  $-8x^{6}y^{9}$%
		\item   $8x^{6}y^{9}$
	\end{enumerate}
\else
\fi

\ifgridin
  $-8x^{6}y^{9}$%
		
\else
\fi

