 \begin{center}
\begin{tikzpicture}\begin{axis}[axis lines=center, xmin=-5, xmax=5, xtick={-4, -2, ..., 4},ytick={0},xlabel={$x$}, ylabel={$y$},ymin=-10,minor x tick num=1,]
\addplot [domain=-5:5, samples=91,smooth,]{(x+3)*(x-2)*(x-1)^2*(-1)};
\end{axis}\end{tikzpicture}\end{center}
If the graph above represents a polynomial function $p(x)$ of degree $4$, which of the following equations could be the equation of $p(x)$?


\ifsat
	\begin{enumerate}[label=\Alph*)]
		\item $p(x)=-2(x+3)(x-2)(x-1)^2 $ % 
		\item $p(x)=-\frac{1}{2}(x+3)^2(x-1)(x-2) $ 
		\item $p(x)=(x+3)(x-2)(x-1)^2 $ 
		\item $p(x)=\frac{1}{2}(x+3)^2(x-1)(x-2) $
	\end{enumerate}
\else
\fi

\ifacteven
	\begin{enumerate}[label=\textbf{\Alph*.},itemsep=\fill,align=left]
		\setcounter{enumii}{5}
		\item $p(x)=-2(x+3)(x-2)(x-1)^2 $ % 
		\item $p(x)=-\frac{1}{2}(x+3)^2(x-1)(x-2) $ 
		\item $p(x)=(x+3)(x-2)(x-1)^2 $ 
		\addtocounter{enumii}{1}
		\item $p(x)=\frac{1}{2}(x+3)^2(x-1)(x-2) $
		\item None of these. 
	\end{enumerate}
\else
\fi

\ifactodd
	\begin{enumerate}[label=\textbf{\Alph*.},itemsep=\fill,align=left]
		\item $p(x)=-2(x+3)(x-2)(x-1)^2 $ % 
		\item $p(x)=-\frac{1}{2}(x+3)^2(x-1)(x-2) $ 
		\item $p(x)=(x+3)(x-2)(x-1)^2 $ 
		\item $p(x)=\frac{1}{2}(x+3)^2(x-1)(x-2) $
		\item None of these. 
	\end{enumerate}
\else
\fi

\ifgridin
 $p(x)=-2(x+3)(x-2)(x-1)^2 $ % 
		
\else
\fi

