 
Simplify: $$ \frac{3}{w-3}-\frac{4}{w-1}$$


\ifsat
	\begin{enumerate}[label=\Alph*)]
		\item {\Large$\frac{w-9}{(x-3)(w-1)} $ }
		\item {\Large$\frac{9-w}{(w-3)(w-1)} $ } % 
		\item {\Large$\frac{-w-9}{(w-3)(w-1)} $}
		\item {\Large$\frac{-3}{w-1} $}
	\end{enumerate}
\else
\fi

\ifacteven
	\begin{enumerate}[label=\textbf{\Alph*.},itemsep=\fill,align=left]
		\setcounter{enumii}{5}
		\item {\Large$\frac{w-9}{(x-3)(w-1)} $ }
		\item {\Large$\frac{9-w}{(w-3)(w-1)} $ } % 
		\item {\Large$\frac{-w-9}{(w-3)(w-1)} $}
		\addtocounter{enumii}{1}
		\item {\Large$\frac{-3}{w-1} $}
		\item None of these. 
	\end{enumerate}
\else
\fi

\ifactodd
	\begin{enumerate}[label=\textbf{\Alph*.},itemsep=\fill,align=left]
		\item {\Large$\frac{w-9}{(x-3)(w-1)} $ }
		\item {\Large$\frac{9-w}{(w-3)(w-1)} $ } % 
		\item {\Large$\frac{-w-9}{(w-3)(w-1)} $}
		\item {\Large$\frac{-3}{w-1} $}
		\item None of these. 
	\end{enumerate}
\else
\fi

\ifgridin
 {\Large$\frac{9-w}{(w-3)(w-1)} $ } % 
		
\else
\fi

